chore: reorg

CollapsingTowers/TwoLevelRec/OperationalSemantics/SmallStep.lean
@@ -1,4 +1,4 @@
-import CollapsingTowers.TwoLevelBasic.Semantic.EvalCtx
+import CollapsingTowers.TwoLevelRec.OperationalSemantics.EvalCtx
 
 inductive head : Expr → Expr → Prop where
   | lets : ∀ e v, value v → head (.lets v e) (opening 0 v e)
@@ -9,6 +9,9 @@ inductive head : Expr → Expr → Prop where
   | lam𝕔 : ∀ e, head (.lam𝕔 (.code e)) (.reflect (.lam e))
   | lets𝕔 : ∀ b e, head (.lets𝕔 b (.code e)) (.code (.lets b e))
   | run : ∀ e, head (.run (.code e)) e
+  -- fix F ↦ λx.F(fix F)(x)
+  | fix₁ : ∀ f, value f → head (.fix₁ f) (.lam (.app₁ (.app₁ f (.fix₁ f)) (.bvar 0)))
+  | fix₂ : ∀ f, head (.fix₂ (.code f)) (.reflect (.fix₁ f))
 
 inductive step_lvl (lvl : ℕ) : Expr → Expr → Prop where
   | pure : ∀ M e₀ e₁, ctx𝕄 lvl M → lc e₀ → head e₀ e₁ → step_lvl lvl M⟦e₀⟧ M⟦e₁⟧
@@ -33,6 +36,12 @@ inductive pure_stepn : Expr → Expr → Prop
 
 notation:max e₀ " ⇾* " e₁  => pure_stepn e₀ e₁
 
+inductive pure_stepn_indexed : ℕ → Expr → Expr → Prop
+  | refl : ∀ e, pure_stepn_indexed 0 e e
+  | multi : ∀ k e₀ e₁ e₂, (e₀ ⇾ e₁) → pure_stepn_indexed k e₁ e₂ → pure_stepn_indexed (k + 1) e₀ e₂
+
+notation:max e₀ " ⇾ " "⟦" k "⟧ " e₁  => pure_stepn_indexed k e₀ e₁
+
 lemma pure_step_impl_step : ∀ e₀ e₁, (e₀ ⇾ e₁) → (e₀ ⇝ e₁) :=
   by
   intros e₀ e₁ Hstep
@@ -50,6 +59,17 @@ lemma pure_stepn_impl_stepn : ∀ e₀ e₁, (e₀ ⇾* e₁) → (e₀ ⇝* e�
     apply stepn.multi
     apply pure_step_impl_step; apply H
     apply IH
+
+lemma pure_stepn_impl_pure_stepn_indexed : ∀ e₀ e₁, (e₀ ⇾* e₁) → ∃ k, (e₀ ⇾ ⟦k⟧ e₁) :=
+  by
+  intros e₀ e₁ Hstepn
+  induction Hstepn
+  case refl => exists 0; apply pure_stepn_indexed.refl
+  case multi H _ IH =>
+    have ⟨k, IH⟩ := IH
+    exists k + 1
+    apply pure_stepn_indexed.multi
+    apply H; apply IH
 
 lemma pure_stepn.trans : ∀ e₀ e₁ e₂, (e₀ ⇾* e₁) → (e₁ ⇾* e₂) → (e₀ ⇾* e₂) :=
   by
@@ -72,16 +92,23 @@ lemma head.fv_shrink : ∀ e₀ e₁, head e₀ e₁ → fv e₁ ⊆ fv e₀ :=
   case lift_lam =>
     rw [← fv.under_maping𝕔]
 
-lemma lc.under_pure_step : ∀ e₀ e₁, pure_step e₀ e₁ → lc e₀ :=
+lemma lc.under_pure_step : ∀ e₀ e₁, (e₀ ⇾ e₁) → lc e₀ :=
   by
   intros e₀ e₁ Hstep
   cases Hstep
   case pure HM Hlc Hhead =>
     apply lc.under_ctx𝕄; apply HM; apply Hlc
 
-lemma lc.under_pure_stepn : ∀ e₀ e₁, pure_stepn e₀ e₁ → lc e₁ → lc e₀ :=
+lemma lc.under_pure_stepn : ∀ e₀ e₁, (e₀ ⇾* e₁) → lc e₁ → lc e₀ :=
   by
   intros e₀ e₁ Hstepn Hlc
+  induction Hstepn
+  case refl => apply Hlc
+  case multi H _ IH => apply lc.under_pure_step; apply H
+
+lemma lc.under_pure_stepn_indexed : ∀ e₀ e₁ k, (e₀ ⇾ ⟦k⟧ e₁) → lc e₁ → lc e₀ :=
+  by
+  intros e₀ e₁ k Hstepn Hlc
   induction Hstepn
   case refl => apply Hlc
   case multi H _ IH => apply lc.under_pure_step; apply H
