CollapsingTowers/TwoLevelBasic/Defs.lean
@@ -1,6 +1,6 @@
 import CollapsingTowers.TwoLevelBasic.Syntax.Defs
 import CollapsingTowers.TwoLevelBasic.Utils.Defs
-import CollapsingTowers.TwoLevelBasic.Semantic.Defs
+import CollapsingTowers.TwoLevelBasic.OperationalSemantics.Defs
 import CollapsingTowers.TwoLevelBasic.SyntacticTyping.Defs
 import CollapsingTowers.TwoLevelBasic.Erasure.Defs
 import CollapsingTowers.TwoLevelBasic.CtxEquiv.Defs
