CollapsingTowers/TwoLevelBasic/Semantic/Defs.lean
@@ -1,6 +1,0 @@
-import CollapsingTowers.TwoLevelBasic.Semantic.Value
-import CollapsingTowers.TwoLevelBasic.Semantic.EvalCtx
-import CollapsingTowers.TwoLevelBasic.Semantic.SmallStep
-import CollapsingTowers.TwoLevelBasic.Semantic.Congruence
-import CollapsingTowers.TwoLevelBasic.Semantic.Deterministic
-import CollapsingTowers.TwoLevelBasic.Semantic.Confluence
