CollapsingTowers/TwoLevelRec/Defs.lean
@@ -1,6 +1,6 @@
 import CollapsingTowers.TwoLevelRec.Syntax.Defs
 import CollapsingTowers.TwoLevelRec.Utils.Defs
-import CollapsingTowers.TwoLevelRec.Semantic.Defs
+import CollapsingTowers.TwoLevelRec.OperationalSemantics.Defs
 import CollapsingTowers.TwoLevelRec.SyntacticTyping.Defs
 import CollapsingTowers.TwoLevelRec.Erasure.Defs
 import CollapsingTowers.TwoLevelRec.CtxEquiv.Defs
