CollapsingTowers/TwoLevelRec/OperationalSemantics/Defs.lean
@@ -1,0 +1,7 @@
+import CollapsingTowers.TwoLevelRec.OperationalSemantics.Value
+import CollapsingTowers.TwoLevelRec.OperationalSemantics.EvalCtx
+import CollapsingTowers.TwoLevelRec.OperationalSemantics.SmallStep
+import CollapsingTowers.TwoLevelRec.OperationalSemantics.Congruence
+import CollapsingTowers.TwoLevelRec.OperationalSemantics.Deterministic
+import CollapsingTowers.TwoLevelRec.OperationalSemantics.Confluence
+import CollapsingTowers.TwoLevelRec.OperationalSemantics.Refine
