CollapsingTowers/TwoLevelRec/Semantic/Defs.lean
@@ -1,7 +1,0 @@
-import CollapsingTowers.TwoLevelRec.Semantic.Value
-import CollapsingTowers.TwoLevelRec.Semantic.EvalCtx
-import CollapsingTowers.TwoLevelRec.Semantic.SmallStep
-import CollapsingTowers.TwoLevelRec.Semantic.Congruence
-import CollapsingTowers.TwoLevelRec.Semantic.Deterministic
-import CollapsingTowers.TwoLevelRec.Semantic.Confluence
-import CollapsingTowers.TwoLevelRec.Semantic.Refine
